Phi_Semantics/PhiSem_Variable.thy
@@ -110,16 +110,16 @@ lemma Var_SubjTyp[simp]:
   \<open>EqualAddress (xa \<Ztypecolon> Var var Ta) (xb \<Ztypecolon> Var var Tb)\<close>
   unfolding EqualAddress_def .. *)
 
-lemma [\<phi>reason 1305 for \<open>\<^bold>v\<^bold>i\<^bold>e\<^bold>w ?R \<heavy_comma> ?H \<longmapsto> ?R''' * \<blangle> ?X \<brangle> \<^bold>w\<^bold>i\<^bold>t\<^bold>h ?P  \<^bold><\<^bold>a\<^bold>c\<^bold>t\<^bold>i\<^bold>o\<^bold>n\<^bold>> ToSA \<^bold>@\<^bold>G\<^bold>O\<^bold>A\<^bold>L ?G\<close>]: \<comment> \<open>attempts the immediate cell\<close>
+lemma [\<phi>reason 1305 for \<open>\<^bold>v\<^bold>i\<^bold>e\<^bold>w ?R \<heavy_comma> ?H \<longmapsto> ?R''' * \<blangle> ?X \<brangle> \<^bold>w\<^bold>i\<^bold>t\<^bold>h ?P  \<^bold><\<^bold>a\<^bold>c\<^bold>t\<^bold>i\<^bold>o\<^bold>n\<^bold>> reason_ToSA True ?G\<close>]: \<comment> \<open>attempts the immediate cell\<close>
   " CHK_SUBGOAL G
 \<Longrightarrow> x \<Ztypecolon> T \<^bold>i\<^bold>m\<^bold>p\<^bold>l\<^bold>i\<^bold>e\<^bold>s x' \<Ztypecolon> T' \<^bold>a\<^bold>n\<^bold>d P
-\<Longrightarrow> \<^bold>v\<^bold>i\<^bold>e\<^bold>w R\<heavy_comma> x \<Ztypecolon> Var var T \<longmapsto> R\<heavy_comma> \<blangle> x' \<Ztypecolon> Var var T' \<brangle> \<^bold>w\<^bold>i\<^bold>t\<^bold>h P  \<^bold><\<^bold>a\<^bold>c\<^bold>t\<^bold>i\<^bold>o\<^bold>n\<^bold>> ToSA \<^bold>@\<^bold>G\<^bold>O\<^bold>A\<^bold>L G"
+\<Longrightarrow> \<^bold>v\<^bold>i\<^bold>e\<^bold>w R\<heavy_comma> x \<Ztypecolon> Var var T \<longmapsto> R\<heavy_comma> \<blangle> x' \<Ztypecolon> Var var T' \<brangle> \<^bold>w\<^bold>i\<^bold>t\<^bold>h P  \<^bold><\<^bold>a\<^bold>c\<^bold>t\<^bold>i\<^bold>o\<^bold>n\<^bold>> reason_ToSA True G"
   unfolding GOAL_CTXT_def FOCUS_TAG_def
   by (simp add: Var_view_shift \<phi>frame_view)
 
-lemma [\<phi>reason 1300 for \<open>\<^bold>v\<^bold>i\<^bold>e\<^bold>w ?R \<heavy_comma> ?H \<longmapsto> ?R''' * \<blangle> ?X \<brangle> \<^bold>w\<^bold>i\<^bold>t\<^bold>h ?P  \<^bold><\<^bold>a\<^bold>c\<^bold>t\<^bold>i\<^bold>o\<^bold>n\<^bold>> ToSA' ?mode \<^bold>@\<^bold>G\<^bold>O\<^bold>A\<^bold>L ?G\<close>]: \<comment> \<open>attempts the immediate cell\<close>
+lemma [\<phi>reason 1300 for \<open>\<^bold>v\<^bold>i\<^bold>e\<^bold>w ?R \<heavy_comma> ?H \<longmapsto> ?R''' * \<blangle> ?X \<brangle> \<^bold>w\<^bold>i\<^bold>t\<^bold>h ?P  \<^bold><\<^bold>a\<^bold>c\<^bold>t\<^bold>i\<^bold>o\<^bold>n\<^bold>> reason_ToSA ?mode ?G\<close>]: \<comment> \<open>attempts the immediate cell\<close>
   " CHK_SUBGOAL G
-\<Longrightarrow> \<^bold>v\<^bold>i\<^bold>e\<^bold>w R\<heavy_comma> x \<Ztypecolon> Var var T \<longmapsto> R\<heavy_comma> \<blangle> x \<Ztypecolon> Var var T \<brangle> \<^bold><\<^bold>a\<^bold>c\<^bold>t\<^bold>i\<^bold>o\<^bold>n\<^bold>> ToSA' mode \<^bold>@\<^bold>G\<^bold>O\<^bold>A\<^bold>L G"
+\<Longrightarrow> \<^bold>v\<^bold>i\<^bold>e\<^bold>w R\<heavy_comma> x \<Ztypecolon> Var var T \<longmapsto> R\<heavy_comma> \<blangle> x \<Ztypecolon> Var var T \<brangle> \<^bold><\<^bold>a\<^bold>c\<^bold>t\<^bold>i\<^bold>o\<^bold>n\<^bold>> reason_ToSA mode G"
   unfolding GOAL_CTXT_def FOCUS_TAG_def
   by (simp add: Var_view_shift \<phi>frame_view view_shift_id) 
 
@@ -139,23 +139,23 @@ lemma [\<phi>reason 1200 for \<open>PROP Branch_Convergence_Type_Pattern (Var ?v
   \<open> PROP Branch_Convergence_Type_Pattern (Var v T) (Var v T')\<close>
   unfolding Branch_Convergence_Type_Pattern_def ..
 
-lemma [\<phi>reason 1520 for \<open>\<^bold>v\<^bold>i\<^bold>e\<^bold>w ?R \<heavy_comma> \<^bold>u\<^bold>n\<^bold>i\<^bold>n\<^bold>i\<^bold>t\<^bold>e\<^bold>d \<^bold>v\<^bold>a\<^bold>r[?var] \<longmapsto> ?R' \<heavy_comma> \<blangle> ?x' \<Ztypecolon> \<^bold>v\<^bold>a\<^bold>r[?var] ?T' \<brangle> \<^bold>w\<^bold>i\<^bold>t\<^bold>h ?P \<^bold><\<^bold>a\<^bold>c\<^bold>t\<^bold>i\<^bold>o\<^bold>n\<^bold>> ToSA \<^bold>@\<^bold>G\<^bold>O\<^bold>A\<^bold>L ?G\<close>]:
+lemma [\<phi>reason 1520 for \<open>\<^bold>v\<^bold>i\<^bold>e\<^bold>w ?R \<heavy_comma> \<^bold>u\<^bold>n\<^bold>i\<^bold>n\<^bold>i\<^bold>t\<^bold>e\<^bold>d \<^bold>v\<^bold>a\<^bold>r[?var] \<longmapsto> ?R' \<heavy_comma> \<blangle> ?x' \<Ztypecolon> \<^bold>v\<^bold>a\<^bold>r[?var] ?T' \<brangle> \<^bold>w\<^bold>i\<^bold>t\<^bold>h ?P \<^bold><\<^bold>a\<^bold>c\<^bold>t\<^bold>i\<^bold>o\<^bold>n\<^bold>> reason_ToSA True ?G\<close>]:
     \<comment> \<open>attempts the immediate cell\<close>
   " FAIL TEXT(\<open>Variable\<close> var \<open>has not been initialized.\<close>)
-\<Longrightarrow> \<^bold>v\<^bold>i\<^bold>e\<^bold>w R \<heavy_comma> \<^bold>u\<^bold>n\<^bold>i\<^bold>n\<^bold>i\<^bold>t\<^bold>e\<^bold>d \<^bold>v\<^bold>a\<^bold>r[var] \<longmapsto> R \<heavy_comma> \<blangle> x' \<Ztypecolon> \<^bold>v\<^bold>a\<^bold>r[var] T' \<brangle> \<^bold>w\<^bold>i\<^bold>t\<^bold>h P \<^bold><\<^bold>a\<^bold>c\<^bold>t\<^bold>i\<^bold>o\<^bold>n\<^bold>> ToSA \<^bold>@\<^bold>G\<^bold>O\<^bold>A\<^bold>L G"
+\<Longrightarrow> \<^bold>v\<^bold>i\<^bold>e\<^bold>w R \<heavy_comma> \<^bold>u\<^bold>n\<^bold>i\<^bold>n\<^bold>i\<^bold>t\<^bold>e\<^bold>d \<^bold>v\<^bold>a\<^bold>r[var] \<longmapsto> R \<heavy_comma> \<blangle> x' \<Ztypecolon> \<^bold>v\<^bold>a\<^bold>r[var] T' \<brangle> \<^bold>w\<^bold>i\<^bold>t\<^bold>h P \<^bold><\<^bold>a\<^bold>c\<^bold>t\<^bold>i\<^bold>o\<^bold>n\<^bold>> reason_ToSA True G"
   unfolding GOAL_CTXT_def Action_Tag_def by blast
 
-lemma [\<phi>reason 1500 for \<open>\<^bold>v\<^bold>i\<^bold>e\<^bold>w ?R \<heavy_comma> ?H \<longmapsto> ?R''' * \<blangle> ?x \<Ztypecolon> Var ?var ?T \<brangle> \<^bold>w\<^bold>i\<^bold>t\<^bold>h ?P \<^bold><\<^bold>a\<^bold>c\<^bold>t\<^bold>i\<^bold>o\<^bold>n\<^bold>> ToSA \<^bold>@\<^bold>G\<^bold>O\<^bold>A\<^bold>L ?G\<close>]:
+lemma [\<phi>reason 1500 for \<open>\<^bold>v\<^bold>i\<^bold>e\<^bold>w ?R \<heavy_comma> ?H \<longmapsto> ?R''' * \<blangle> ?x \<Ztypecolon> Var ?var ?T \<brangle> \<^bold>w\<^bold>i\<^bold>t\<^bold>h ?P \<^bold><\<^bold>a\<^bold>c\<^bold>t\<^bold>i\<^bold>o\<^bold>n\<^bold>> reason_ToSA True ?G\<close>]:
     \<comment> \<open>attempts the immediate cell\<close>
   " CHK_SUBGOAL G
 \<Longrightarrow> x \<Ztypecolon> T \<^bold>i\<^bold>m\<^bold>p\<^bold>l\<^bold>i\<^bold>e\<^bold>s x' \<Ztypecolon> T' \<^bold>a\<^bold>n\<^bold>d P
-\<Longrightarrow> \<^bold>v\<^bold>i\<^bold>e\<^bold>w R \<heavy_comma> x \<Ztypecolon> Var var T \<longmapsto> R \<heavy_comma> \<blangle> x' \<Ztypecolon> Var var T' \<brangle> \<^bold>w\<^bold>i\<^bold>t\<^bold>h P \<^bold><\<^bold>a\<^bold>c\<^bold>t\<^bold>i\<^bold>o\<^bold>n\<^bold>> ToSA \<^bold>@\<^bold>G\<^bold>O\<^bold>A\<^bold>L G"
+\<Longrightarrow> \<^bold>v\<^bold>i\<^bold>e\<^bold>w R \<heavy_comma> x \<Ztypecolon> Var var T \<longmapsto> R \<heavy_comma> \<blangle> x' \<Ztypecolon> Var var T' \<brangle> \<^bold>w\<^bold>i\<^bold>t\<^bold>h P \<^bold><\<^bold>a\<^bold>c\<^bold>t\<^bold>i\<^bold>o\<^bold>n\<^bold>> reason_ToSA True G"
   unfolding GOAL_CTXT_def FOCUS_TAG_def
   by (simp add: Var_view_shift \<phi>frame_view)
 
-lemma [\<phi>reason 1450 for \<open>\<^bold>v\<^bold>i\<^bold>e\<^bold>w ?R \<heavy_comma> ?H \<longmapsto> ?R''' * \<blangle> ?x \<Ztypecolon> Var ?var ?T \<brangle> \<^bold>w\<^bold>i\<^bold>t\<^bold>h ?P \<^bold><\<^bold>a\<^bold>c\<^bold>t\<^bold>i\<^bold>o\<^bold>n\<^bold>> ToSA' ?mode \<^bold>@\<^bold>G\<^bold>O\<^bold>A\<^bold>L ?G\<close>]:
-  \<open> \<^bold>v\<^bold>i\<^bold>e\<^bold>w R \<longmapsto> R' \<heavy_comma> \<blangle> x \<Ztypecolon> Var var T \<brangle> \<^bold>w\<^bold>i\<^bold>t\<^bold>h P  \<^bold><\<^bold>a\<^bold>c\<^bold>t\<^bold>i\<^bold>o\<^bold>n\<^bold>> ToSA' mode \<^bold>@\<^bold>G\<^bold>O\<^bold>A\<^bold>L G
-\<Longrightarrow> \<^bold>v\<^bold>i\<^bold>e\<^bold>w R \<heavy_comma> H \<longmapsto> R' \<heavy_comma> H \<heavy_comma> \<blangle> x \<Ztypecolon> Var var T \<brangle> \<^bold>w\<^bold>i\<^bold>t\<^bold>h P \<^bold><\<^bold>a\<^bold>c\<^bold>t\<^bold>i\<^bold>o\<^bold>n\<^bold>> ToSA' mode  \<^bold>@\<^bold>G\<^bold>O\<^bold>A\<^bold>L G\<close>
+lemma [\<phi>reason 1450 for \<open>\<^bold>v\<^bold>i\<^bold>e\<^bold>w ?R \<heavy_comma> ?H \<longmapsto> ?R''' * \<blangle> ?x \<Ztypecolon> Var ?var ?T \<brangle> \<^bold>w\<^bold>i\<^bold>t\<^bold>h ?P \<^bold><\<^bold>a\<^bold>c\<^bold>t\<^bold>i\<^bold>o\<^bold>n\<^bold>> reason_ToSA ?mode ?G\<close>]:
+  \<open> \<^bold>v\<^bold>i\<^bold>e\<^bold>w R \<longmapsto> R' \<heavy_comma> \<blangle> x \<Ztypecolon> Var var T \<brangle> \<^bold>w\<^bold>i\<^bold>t\<^bold>h P  \<^bold><\<^bold>a\<^bold>c\<^bold>t\<^bold>i\<^bold>o\<^bold>n\<^bold>> reason_ToSA mode G
+\<Longrightarrow> \<^bold>v\<^bold>i\<^bold>e\<^bold>w R \<heavy_comma> H \<longmapsto> R' \<heavy_comma> H \<heavy_comma> \<blangle> x \<Ztypecolon> Var var T \<brangle> \<^bold>w\<^bold>i\<^bold>t\<^bold>h P \<^bold><\<^bold>a\<^bold>c\<^bold>t\<^bold>i\<^bold>o\<^bold>n\<^bold>> reason_ToSA mode G\<close>
   using ToSA_skip[OF CHK_SUBGOAL_I] .
 
 
