Phi_System/PhiSem_Formalization_Tools.thy
@@ -315,8 +315,8 @@ lemma ToSA_by_structural_extraction:
 \<Longrightarrow> SUBGOAL G G2
 \<Longrightarrow> (Q' \<Longrightarrow> Try Any (Structural_Extract (y \<Ztypecolon> \<phi> U) R1 (x \<Ztypecolon> \<phi> T) W P2)  \<^bold>@\<^bold>G\<^bold>O\<^bold>A\<^bold>L G2)
 \<Longrightarrow> SOLVE_SUBGOAL G2
-\<Longrightarrow> \<^bold>v\<^bold>i\<^bold>e\<^bold>w A \<longmapsto> R2 \<heavy_comma> \<blangle> W \<brangle> \<^bold>w\<^bold>i\<^bold>t\<^bold>h P1 \<^bold><\<^bold>a\<^bold>c\<^bold>t\<^bold>i\<^bold>o\<^bold>n\<^bold>> ToSA \<^bold>@\<^bold>G\<^bold>O\<^bold>A\<^bold>L G
-\<Longrightarrow> \<^bold>v\<^bold>i\<^bold>e\<^bold>w A \<heavy_comma> y \<Ztypecolon> \<phi> U \<longmapsto> R2\<heavy_comma> R1\<heavy_comma> \<blangle> x \<Ztypecolon> \<phi> T \<brangle> \<^bold>w\<^bold>i\<^bold>t\<^bold>h P1 \<and> P2 \<^bold><\<^bold>a\<^bold>c\<^bold>t\<^bold>i\<^bold>o\<^bold>n\<^bold>> ToSA \<^bold>@\<^bold>G\<^bold>O\<^bold>A\<^bold>L G"
+\<Longrightarrow> \<^bold>v\<^bold>i\<^bold>e\<^bold>w A \<longmapsto> R2 \<heavy_comma> \<blangle> W \<brangle> \<^bold>w\<^bold>i\<^bold>t\<^bold>h P1 \<^bold><\<^bold>a\<^bold>c\<^bold>t\<^bold>i\<^bold>o\<^bold>n\<^bold>> reason_ToSA True G
+\<Longrightarrow> \<^bold>v\<^bold>i\<^bold>e\<^bold>w A \<heavy_comma> y \<Ztypecolon> \<phi> U \<longmapsto> R2\<heavy_comma> R1\<heavy_comma> \<blangle> x \<Ztypecolon> \<phi> T \<brangle> \<^bold>w\<^bold>i\<^bold>t\<^bold>h P1 \<and> P2 \<^bold><\<^bold>a\<^bold>c\<^bold>t\<^bold>i\<^bold>o\<^bold>n\<^bold>> reason_ToSA True G"
   unfolding Premise_def GOAL_CTXT_def FOCUS_TAG_def Structural_Extract_def Simplify_def Action_Tag_def Try_def
   \<medium_left_bracket> premises SI and Q and _ and SE and _ and A
     have \<open>Q'\<close> using \<phi> SI[unfolded Structure_Info_def] Q by blast
@@ -336,10 +336,10 @@ lemma ToSA_by_structural_extraction__reverse_morphism:
             \<^bold>@\<^bold>G\<^bold>O\<^bold>A\<^bold>L G2)
 \<Longrightarrow> SOLVE_SUBGOAL G2
 \<Longrightarrow> \<^bold>v\<^bold>i\<^bold>e\<^bold>w A \<longmapsto> R2 \<heavy_comma> \<blangle> W \<brangle> \<^bold>w\<^bold>i\<^bold>t\<^bold>h (Automatic_Morphism RP1 (\<^bold>v\<^bold>i\<^bold>e\<^bold>w R2'\<heavy_comma> \<blangle> W' \<brangle> \<longmapsto> A' \<^bold>w\<^bold>i\<^bold>t\<^bold>h P1') \<and> P1)
-    \<^bold><\<^bold>a\<^bold>c\<^bold>t\<^bold>i\<^bold>o\<^bold>n\<^bold>> ToSA \<^bold>@\<^bold>G\<^bold>O\<^bold>A\<^bold>L G
+    \<^bold><\<^bold>a\<^bold>c\<^bold>t\<^bold>i\<^bold>o\<^bold>n\<^bold>> reason_ToSA True G
 \<Longrightarrow> \<^bold>v\<^bold>i\<^bold>e\<^bold>w A \<heavy_comma> y \<Ztypecolon> \<phi> U \<longmapsto> R2\<heavy_comma> R1\<heavy_comma> \<blangle> x \<Ztypecolon> \<phi> T \<brangle> \<^bold>w\<^bold>i\<^bold>t\<^bold>h
       (Automatic_Morphism (RP2 \<and>\<^sub>\<r> RP1) (\<^bold>v\<^bold>i\<^bold>e\<^bold>w R2'\<heavy_comma> R1'\<heavy_comma> \<blangle> x' \<Ztypecolon> \<phi> T' \<brangle> \<longmapsto> A'\<heavy_comma> y' \<Ztypecolon> \<phi> U' \<^bold>w\<^bold>i\<^bold>t\<^bold>h P1' \<and> P2') \<and> P1 \<and> P2)
-    \<^bold><\<^bold>a\<^bold>c\<^bold>t\<^bold>i\<^bold>o\<^bold>n\<^bold>> ToSA \<^bold>@\<^bold>G\<^bold>O\<^bold>A\<^bold>L G"
+    \<^bold><\<^bold>a\<^bold>c\<^bold>t\<^bold>i\<^bold>o\<^bold>n\<^bold>> reason_ToSA True G"
   unfolding Premise_def GOAL_CTXT_def FOCUS_TAG_def Structural_Extract_def Simplify_def
             Action_Tag_def Morphism_def Compact_Antecedent_def Try_def GOAL_CTXT_def
   \<medium_left_bracket> premises SI and Q and _ and SE and _ and A
@@ -355,12 +355,12 @@ lemma ToSA_by_structural_extraction__reverse_morphism:
 
 
 lemma ToSA_skip [\<phi>reason 1200
-    for \<open>\<^bold>v\<^bold>i\<^bold>e\<^bold>w ?R \<heavy_comma> ?X \<longmapsto> ?R'\<heavy_comma> \<blangle> ?x \<Ztypecolon> \<phi> ?T \<brangle> \<^bold>w\<^bold>i\<^bold>t\<^bold>h ?P \<^bold><\<^bold>a\<^bold>c\<^bold>t\<^bold>i\<^bold>o\<^bold>n\<^bold>> ToSA' ?mode \<^bold>@\<^bold>G\<^bold>O\<^bold>A\<^bold>L ?G\<close>
-    except \<open>\<^bold>v\<^bold>i\<^bold>e\<^bold>w ?R \<heavy_comma> ?y \<Ztypecolon> \<phi> ?U \<longmapsto> ?R'\<heavy_comma> \<blangle> ?x \<Ztypecolon> \<phi> ?T \<brangle> \<^bold>w\<^bold>i\<^bold>t\<^bold>h ?P \<^bold><\<^bold>a\<^bold>c\<^bold>t\<^bold>i\<^bold>o\<^bold>n\<^bold>> ToSA' ?mode \<^bold>@\<^bold>G\<^bold>O\<^bold>A\<^bold>L ?G\<close>
+    for \<open>\<^bold>v\<^bold>i\<^bold>e\<^bold>w ?R \<heavy_comma> ?X \<longmapsto> ?R'\<heavy_comma> \<blangle> ?x \<Ztypecolon> \<phi> ?T \<brangle> \<^bold>w\<^bold>i\<^bold>t\<^bold>h ?P \<^bold><\<^bold>a\<^bold>c\<^bold>t\<^bold>i\<^bold>o\<^bold>n\<^bold>> reason_ToSA ?mode ?G\<close>
+    except \<open>\<^bold>v\<^bold>i\<^bold>e\<^bold>w ?R \<heavy_comma> ?y \<Ztypecolon> \<phi> ?U \<longmapsto> ?R'\<heavy_comma> \<blangle> ?x \<Ztypecolon> \<phi> ?T \<brangle> \<^bold>w\<^bold>i\<^bold>t\<^bold>h ?P \<^bold><\<^bold>a\<^bold>c\<^bold>t\<^bold>i\<^bold>o\<^bold>n\<^bold>> reason_ToSA ?mode ?G\<close>
 ]:
-  " \<^bold>v\<^bold>i\<^bold>e\<^bold>w R \<longmapsto> R'\<heavy_comma> \<blangle> x \<Ztypecolon> \<phi> T \<brangle> \<^bold>w\<^bold>i\<^bold>t\<^bold>h P \<^bold><\<^bold>a\<^bold>c\<^bold>t\<^bold>i\<^bold>o\<^bold>n\<^bold>> ToSA' mode \<^bold>@\<^bold>G\<^bold>O\<^bold>A\<^bold>L G
-\<Longrightarrow> \<^bold>v\<^bold>i\<^bold>e\<^bold>w R \<heavy_comma> X \<longmapsto> R'\<heavy_comma> X\<heavy_comma> \<blangle> x \<Ztypecolon> \<phi> T \<brangle> \<^bold>w\<^bold>i\<^bold>t\<^bold>h P \<^bold><\<^bold>a\<^bold>c\<^bold>t\<^bold>i\<^bold>o\<^bold>n\<^bold>> ToSA' mode \<^bold>@\<^bold>G\<^bold>O\<^bold>A\<^bold>L G"
-  unfolding cast_def split_paired_All Action_Tag_def
+  " \<^bold>v\<^bold>i\<^bold>e\<^bold>w R \<longmapsto> R'\<heavy_comma> \<blangle> x \<Ztypecolon> \<phi> T \<brangle> \<^bold>w\<^bold>i\<^bold>t\<^bold>h P \<^bold><\<^bold>a\<^bold>c\<^bold>t\<^bold>i\<^bold>o\<^bold>n\<^bold>> reason_ToSA mode G
+\<Longrightarrow> \<^bold>v\<^bold>i\<^bold>e\<^bold>w R \<heavy_comma> X \<longmapsto> R'\<heavy_comma> X\<heavy_comma> \<blangle> x \<Ztypecolon> \<phi> T \<brangle> \<^bold>w\<^bold>i\<^bold>t\<^bold>h P \<^bold><\<^bold>a\<^bold>c\<^bold>t\<^bold>i\<^bold>o\<^bold>n\<^bold>> reason_ToSA mode G"
+  unfolding Action_Tag_def FOCUS_TAG_def split_paired_All Action_Tag_def
   by (smt (verit) \<phi>view_shift_intro_frame_R mult.assoc mult.commute)
 
 
@@ -412,7 +412,7 @@ lemma [\<phi>reason 1200 for
 
 lemma [\<phi>reason for \<open>\<^bold>p\<^bold>r\<^bold>o\<^bold>c ?f \<lbrace> ?S1 \<longmapsto> \<lambda>ret. ?S2\<heavy_comma> SYNTHESIS ?x \<Ztypecolon> \<phi> ?T \<^bold>t\<^bold>h\<^bold>r\<^bold>o\<^bold>w\<^bold>s ?E \<rbrace> \<^bold>@\<^bold>G\<^bold>O\<^bold>A\<^bold>L ?G\<close>]:
   \<open> SUBGOAL G G'
-\<Longrightarrow> \<^bold>v\<^bold>i\<^bold>e\<^bold>w S1 \<longmapsto> S2\<heavy_comma> \<blangle> x \<Ztypecolon> \<phi> T \<brangle> \<^bold><\<^bold>a\<^bold>c\<^bold>t\<^bold>i\<^bold>o\<^bold>n\<^bold>> ToSA \<^bold>@\<^bold>G\<^bold>O\<^bold>A\<^bold>L G'
+\<Longrightarrow> \<^bold>v\<^bold>i\<^bold>e\<^bold>w S1 \<longmapsto> S2\<heavy_comma> \<blangle> x \<Ztypecolon> \<phi> T \<brangle> \<^bold><\<^bold>a\<^bold>c\<^bold>t\<^bold>i\<^bold>o\<^bold>n\<^bold>> reason_ToSA True G'
 \<Longrightarrow> SOLVE_SUBGOAL G'
 \<Longrightarrow> \<^bold>p\<^bold>r\<^bold>o\<^bold>c Return \<phi>V_none \<lbrace> S1 \<longmapsto> \<lambda>_. S2\<heavy_comma> SYNTHESIS x \<Ztypecolon> \<phi> T \<rbrace> \<^bold>@\<^bold>G\<^bold>O\<^bold>A\<^bold>L G\<close>
   unfolding GOAL_CTXT_def FOCUS_TAG_def Synthesis_def Action_Tag_def
@@ -522,10 +522,10 @@ lemma partial_implies_raw:
 paragraph \<open>Reasoning Rules\<close>
 
 declare ToSA_by_structural_extraction
-    [\<phi>reason 1210 for \<open>\<^bold>v\<^bold>i\<^bold>e\<^bold>w ?A \<heavy_comma> ?y \<Ztypecolon> \<phi> ?U \<longmapsto> ?R \<heavy_comma> \<blangle> ?x \<Ztypecolon> \<phi> ?T \<brangle> \<^bold>w\<^bold>i\<^bold>t\<^bold>h ?P \<^bold><\<^bold>a\<^bold>c\<^bold>t\<^bold>i\<^bold>o\<^bold>n\<^bold>> ToSA \<^bold>@\<^bold>G\<^bold>O\<^bold>A\<^bold>L ?G\<close>]
+    [\<phi>reason 1210 for \<open>\<^bold>v\<^bold>i\<^bold>e\<^bold>w ?A \<heavy_comma> ?y \<Ztypecolon> \<phi> ?U \<longmapsto> ?R \<heavy_comma> \<blangle> ?x \<Ztypecolon> \<phi> ?T \<brangle> \<^bold>w\<^bold>i\<^bold>t\<^bold>h ?P \<^bold><\<^bold>a\<^bold>c\<^bold>t\<^bold>i\<^bold>o\<^bold>n\<^bold>> reason_ToSA True ?G\<close>]
 declare ToSA_by_structural_extraction__reverse_morphism
     [\<phi>reason 1213 for \<open>\<^bold>v\<^bold>i\<^bold>e\<^bold>w ?A \<heavy_comma> ?y \<Ztypecolon> \<phi> ?U \<longmapsto> ?R \<heavy_comma> \<blangle> ?x \<Ztypecolon> \<phi> ?T \<brangle> \<^bold>w\<^bold>i\<^bold>t\<^bold>h (Automatic_Morphism ?RP ?RX \<and> ?P)
-                        \<^bold><\<^bold>a\<^bold>c\<^bold>t\<^bold>i\<^bold>o\<^bold>n\<^bold>> ToSA \<^bold>@\<^bold>G\<^bold>O\<^bold>A\<^bold>L ?G\<close>]
+                       \<^bold><\<^bold>a\<^bold>c\<^bold>t\<^bold>i\<^bold>o\<^bold>n\<^bold>> reason_ToSA True ?G\<close>]
 
 end
 
@@ -628,10 +628,10 @@ lemma expand:
     using expand_subj[where r=r and x=x, simplified prems(2) Subjection_True, OF prems(1)] . .
 
 declare ToSA_by_structural_extraction
-   [\<phi>reason 1210 for \<open>\<^bold>v\<^bold>i\<^bold>e\<^bold>w ?A \<heavy_comma> ?y \<Ztypecolon> \<phi> ?U \<longmapsto> ?R \<heavy_comma> \<blangle> ?x \<Ztypecolon> \<phi> ?T \<brangle> \<^bold>w\<^bold>i\<^bold>t\<^bold>h ?P \<^bold><\<^bold>a\<^bold>c\<^bold>t\<^bold>i\<^bold>o\<^bold>n\<^bold>> ToSA \<^bold>@\<^bold>G\<^bold>O\<^bold>A\<^bold>L ?G\<close>]
+   [\<phi>reason 1210 for \<open>\<^bold>v\<^bold>i\<^bold>e\<^bold>w ?A \<heavy_comma> ?y \<Ztypecolon> \<phi> ?U \<longmapsto> ?R \<heavy_comma> \<blangle> ?x \<Ztypecolon> \<phi> ?T \<brangle> \<^bold>w\<^bold>i\<^bold>t\<^bold>h ?P \<^bold><\<^bold>a\<^bold>c\<^bold>t\<^bold>i\<^bold>o\<^bold>n\<^bold>> reason_ToSA True ?G\<close>]
 declare ToSA_by_structural_extraction__reverse_morphism
    [\<phi>reason 1213 for \<open>\<^bold>v\<^bold>i\<^bold>e\<^bold>w ?A \<heavy_comma> ?y \<Ztypecolon> \<phi> ?U \<longmapsto> ?R \<heavy_comma> \<blangle> ?x \<Ztypecolon> \<phi> ?T \<brangle> \<^bold>w\<^bold>i\<^bold>t\<^bold>h (Automatic_Morphism ?RP ?RX \<and> ?P)
-        \<^bold><\<^bold>a\<^bold>c\<^bold>t\<^bold>i\<^bold>o\<^bold>n\<^bold>> ToSA \<^bold>@\<^bold>G\<^bold>O\<^bold>A\<^bold>L ?G\<close>]
+        \<^bold><\<^bold>a\<^bold>c\<^bold>t\<^bold>i\<^bold>o\<^bold>n\<^bold>> reason_ToSA True ?G\<close>]
 
 end
 
@@ -713,10 +713,10 @@ paragraph \<open>\<phi>-Type\<close>
 abbreviation \<open>\<phi>_ag T \<equiv> \<phi> (Agreement (Nonsepable T))\<close>
 
 declare ToSA_by_structural_extraction
-    [\<phi>reason 1210 for \<open>\<^bold>v\<^bold>i\<^bold>e\<^bold>w ?A \<heavy_comma> ?y \<Ztypecolon> \<phi> ?U \<longmapsto> ?R \<heavy_comma> \<blangle> ?x \<Ztypecolon> \<phi> ?T \<brangle> \<^bold>w\<^bold>i\<^bold>t\<^bold>h ?P \<^bold><\<^bold>a\<^bold>c\<^bold>t\<^bold>i\<^bold>o\<^bold>n\<^bold>> ToSA \<^bold>@\<^bold>G\<^bold>O\<^bold>A\<^bold>L ?G\<close>]
+    [\<phi>reason 1210 for \<open>\<^bold>v\<^bold>i\<^bold>e\<^bold>w ?A \<heavy_comma> ?y \<Ztypecolon> \<phi> ?U \<longmapsto> ?R \<heavy_comma> \<blangle> ?x \<Ztypecolon> \<phi> ?T \<brangle> \<^bold>w\<^bold>i\<^bold>t\<^bold>h ?P \<^bold><\<^bold>a\<^bold>c\<^bold>t\<^bold>i\<^bold>o\<^bold>n\<^bold>> reason_ToSA True ?G\<close>]
 declare ToSA_by_structural_extraction__reverse_morphism
     [\<phi>reason 1213 for \<open>\<^bold>v\<^bold>i\<^bold>e\<^bold>w ?A \<heavy_comma> ?y \<Ztypecolon> \<phi> ?U \<longmapsto> ?R \<heavy_comma> \<blangle> ?x \<Ztypecolon> \<phi> ?T \<brangle> \<^bold>w\<^bold>i\<^bold>t\<^bold>h (Automatic_Morphism ?RP ?RX \<and> ?P)
-        \<^bold><\<^bold>a\<^bold>c\<^bold>t\<^bold>i\<^bold>o\<^bold>n\<^bold>> ToSA \<^bold>@\<^bold>G\<^bold>O\<^bold>A\<^bold>L ?G\<close>]
+        \<^bold><\<^bold>a\<^bold>c\<^bold>t\<^bold>i\<^bold>o\<^bold>n\<^bold>> reason_ToSA True ?G\<close>]
 
 lemma \<phi>_double_\<phi>app:
   \<open>\<^bold>v\<^bold>i\<^bold>e\<^bold>w x \<Ztypecolon> \<phi>_ag T \<longmapsto> x \<Ztypecolon> \<phi>_ag T \<heavy_comma> x \<Ztypecolon> \<phi>_ag T\<close>
